---
layout: post
title:  "Deriving the Additive Identity from the Pythagorean Theorem"
date:   2021-09-27 09:49:00 +0500
categories: math proof pythagoream polarform
---

$$\require{cancel}$$

Following is a whimsical proof which performs some algebraic gymnastics to prove that $$ sin^2 \theta + cos^2 \theta = 1 $$ using the Pythagorean Theorem, and is readable enough for 5th graders (i hope)...

## Statement to Prove

$$ a^2 + b^2 = c^2 \longleftrightarrow sin^2 \theta + cos^2 \theta $$

## Proof

### Components

The equation $$ sin^2 \theta + cos^2 \theta = 1 $$ has three individual components we need to bring out from $$ a^2 + b^2 = c^2 $$. The first component is the Additive Identity $$ 1 $$ which will be easy to bring out in most cases (including this one). The second and third components are the "squares".

### Reasoning

Pythagorean Theorem =  $$ a^2 + b^2 = c^2 $$

> First we will Pick one side (Say the right side) and divide it by itself to get $$ 1 $$. In our case we will be dividing $$ c^2 $$ by $$ c^2 $$. Also, we will be dividing $$ c^2 $$ from both sides to keep the equation balanced.

$$ \longrightarrow \frac{a^2 + b^2}{c^2} = \frac{c^2}{c^2} $$

$$ \longrightarrow \frac{a^2 + b^2}{c^2} = 1 $$

$$ \longrightarrow \frac{a^2}{c^2} + \frac{b^2}{c^2} = 1 $$

$$ \longrightarrow (\frac{a}{c})^2 + (\frac{b}{c})^2 = 1 $$

> We have lead our equation in this direction because we need the two "square" components. 

$$ \longrightarrow (cos \theta)^2 + (sin \theta)^2 = 1 $$

$$ \longrightarrow cos^2 \theta + sin^2 \theta = 1 $$

$$ \longrightarrow sin^2 \theta + cos^2 \theta = 1 $$

$$ \text{Q.E.D} $$

> All steps are reversable, hence the proof works backwards too!

Similarly we can also begin by taking the left side for the additive identity:-

$$ \longrightarrow \frac{a^2 + b^2}{a^2 + b^2} = \frac{c^2}{a^2 + b^2 } $$

$$ \longrightarrow 1 = \frac{c^2}{a^2 + b^2 } $$

$$ \longrightarrow 1 = \frac{ a^2 + b^2 }{ c^2 } $$

$$ \longrightarrow \frac{ a^2 + b^2 }{ c^2 } = 1 $$

$$ \longrightarrow \frac{a^2}{c^2} + \frac{b^2}{c^2} = 1 $$

$$ \longrightarrow (\frac{a}{c})^2 + (\frac{b}{c})^2 = 1 $$

> We have lead our equation in this direction because we need the two "square" components. 

$$ \longrightarrow (cos \theta)^2 + (sin \theta)^2 = 1 $$

$$ \longrightarrow cos^2 \theta + sin^2 \theta = 1 $$

$$ \longrightarrow sin^2 \theta + cos^2 \theta = 1 $$

$$ \text{Q.E.D} $$

> All steps are reversable, hence the proof works backwards too!

> The Proof was written by Ray Voice as an original work and publication. It was published in the book "A Complete guide to Mathamatics" by Ray Voice and Anna Voice, comming soon to international markets.

<script src="https://cdn.mathjax.org/mathjax/latest/MathJax.js?config=TeX-AMS-MML_HTMLorMML" type="text/javascript"></script>

